theories/Eq/SimUpToTaus.v
@@ -192,13 +192,14 @@ Lemma sutt_bind' {E R1 R2 S1 S2} {RR: R1 -> R2 -> Prop} {SS: S1 -> S2 -> Prop}:
                   @sutt E _ _ SS (ITree.bind t1 s1) (ITree.bind t2 s2).
 Proof.
   pcofix self. pstep. intros.
-  punfold H0.
-  rewrite 2 unfold_bind_.
+  punfold H0. unfold observe; cbn.
   induction H0; intros.
   - simpl. apply H1 in H. punfold H. eapply monotone_suttF; eauto using upaco2_mon_bot.
   - simpl. pclearbot. econstructor. eauto.
   - constructor. eauto with paco.
-  - constructor. pclearbot. rewrite (itree_eta' ot2), <- unfold_bind_. eauto.
+  - constructor. pclearbot.
+    right. specialize (self t0 (go ot2) EQTAUS _ _ H1).
+    apply self.
 Qed.
 
 Require Import Coq.Relations.Relations.
